Invariant/ValidAttacker/ValidAttackerI/AbuseElevationControlMechanism.v
@@ -1,0 +1,143 @@
+Require Import Coq.Lists.List.
+
+Require Import Machine.Machine.
+Require Import Machine.MachineValid.
+Require Import Machine.MachineAuxFunctions.
+Require Import Attacker.Attacker.
+Require Import Technique.Technique.
+Require Import Technique.TechniquePreCondition.
+Require Import Technique.TechniquePostCondition.
+
+Require Import Invariant.AuxLemmas.AuxLemmasMachineUser.
+Require Import Invariant.AuxLemmas.AuxLemmasEnviroment.
+Require Import Invariant.AuxLemmas.AuxLemmasAccount.
+Require Import Invariant.AuxTactics.
+
+Lemma one_step_abuse_elevation_control_mechanism_preserves_valid_attacker_i : forall (a a' : Attacker) (n: network_map) (aValid: valid_attacker a n) (m : idMachine) (u: idUser),
+      valid_concrete_network n -> Pre a (Abuse_Elevation_Control_Mechanism m u) -> Post a (Abuse_Elevation_Control_Mechanism m u) n a' -> valid_attacker_i a'.
+  Proof.
+    intros a a' network validAttacker m u validNetwork pre post.
+    unfold valid_attacker_i.
+    intros m0 u0 H_known_machines_a'.
+    elim_intro_clear validAttacker validAttackerI validAttacker'.
+    unfold Pre in pre; unfold Post in post.
+    clear validNetwork validAttacker'.
+
+    elim_intro_clear post Hsecrets post'.
+    elim_intro_clear post' Hmastered post.
+    elim_intro_clear post mac post'.
+    elim_intro_clear post' macView post.
+    elim_intro_clear post newMacView post'.
+    elim_intro_clear post' u' post.
+    elim_intro_clear post newAccountsView post'.
+    elim_intro_clear post' accHigh post.
+    elim_intro_clear post accHighView post'.
+
+    elim_intro_clear post' network_m post.
+    elim_intro_clear post env_macView post'.
+    elim_intro_clear post' Hin_accs post.
+    elim_intro_clear post HaccHigh_user post'.
+    elim_intro_clear post' HaccHigh_service post.
+    elim_intro_clear post HaccHigh_priv post'.
+    elim_intro_clear post' HaccHighView_eq post.
+    elim_intro_clear post newAccountsView_eq post'.
+    elim_intro_clear post' newMacView_eq post.
+    elim_intro_clear post known_machines_a' env_a'.
+
+    unfold valid_attacker_i in validAttackerI.
+    rewrite known_machines_a' in H_known_machines_a'.
+    apply member_add_machine_user in H_known_machines_a'.
+    case (idMachine_eq m0 m); case (idUser_eq u0 u'); intros.
+    - unfold modify_machine in env_a'.
+      rewrite env_a'.
+      case (idMachine_eq m0 m); intro.
+      -- exists newMacView.
+         split.
+         --- reflexivity.
+         --- unfold registered_users.
+             exists accHighView.
+             split.
+             ---- rewrite HaccHighView_eq.
+                  simpl.
+                  symmetry.
+                  exact e.
+             ---- rewrite newMacView_eq.
+                  simpl.
+                  rewrite newAccountsView_eq.
+                  apply member_addAccount.
+                  auto.
+      -- contradiction.
+    - elim (validAttackerI m0 u0).
+      intros MAC IH.
+      elim_intro_clear IH env_MAC users_MAC.
+      -- exists newMacView.
+         split.
+         --- rewrite env_a'.
+             unfold modify_machine.
+             case (idMachine_eq m0 m); intro eq_m.
+             ---- reflexivity.
+             ---- contradiction.
+         --- unfold registered_users.
+             rewrite newMacView_eq.
+             simpl.
+             rewrite newAccountsView_eq.
+             rewrite e in env_MAC.
+             assert (macView = MAC).
+             ---- apply (enviroment_map_image (enviroment a) m macView MAC).
+                  ----- exact env_macView.
+                  ----- exact env_MAC.
+             ---- unfold registered_users in users_MAC.
+                  rewrite <- H in users_MAC.
+                  elim_intro_clear users_MAC acc_u0 users_MAC'.
+                  elim_intro_clear users_MAC' acc_u0_eq acc_In_accounts.
+                  exists acc_u0.
+                  split.
+                  ----- exact acc_u0_eq.
+                  ----- apply addAccount_preserves_membership_when_neq.
+                        ------- rewrite acc_u0_eq.
+                                rewrite HaccHighView_eq.
+                                simpl.
+                                exact n.
+                        ------- exact acc_In_accounts.
+      -- elim H_known_machines_a'.
+         --- intro eq_tuple.
+             injection eq_tuple.
+             intros.
+             symmetry in H.
+             contradiction.
+         --- intro. exact H.
+    - elim (validAttackerI m0 u0).
+      intros MAC IH.
+      elim_intro_clear IH env_MAC users_MAC.
+      exists MAC.
+      split.
+      -- rewrite (enviroment_eq (enviroment a) (enviroment a') m0 m newMacView).
+         --- exact env_MAC.
+         --- exact n.
+         --- exact env_a'.
+      -- exact users_MAC.
+      -- elim H_known_machines_a'.
+         --- intro eq_tuple.
+             injection eq_tuple.
+             intros.
+             symmetry in H0.
+             contradiction.
+         --- intro. exact H.
+    - elim (validAttackerI m0 u0).
+      intros MAC IH.
+      elim_intro_clear IH env_MAC users_MAC.
+      exists MAC.
+      split.
+      -- rewrite (enviroment_eq (enviroment a) (enviroment a') m0 m newMacView).
+         --- exact env_MAC.
+         --- exact n0.
+         --- exact env_a'.
+      -- exact users_MAC.
+      -- elim H_known_machines_a'.
+         --- intro eq_tuple.
+             injection eq_tuple.
+             intros.
+             symmetry in H0.
+             contradiction.
+         --- intro. exact H.
+  Qed.
