Invariant/ValidAttacker/ValidAttackerII/AbuseElevationControlMechanism.v
@@ -1,0 +1,77 @@
+Require Import Coq.Lists.List.
+
+Require Import Machine.Machine.
+Require Import Machine.MachineValid.
+Require Import Machine.MachineAuxFunctions.
+Require Import Attacker.Attacker.
+Require Import Technique.Technique.
+Require Import Technique.TechniquePreCondition.
+Require Import Technique.TechniquePostCondition.
+
+Require Import Invariant.AuxLemmas.AuxLemmasEnviroment.
+Require Import Invariant.AuxTactics.
+
+Lemma one_step_abuse_elevation_control_mechanism_preserves_valid_attacker_ii : forall (a a' : Attacker) (n: network_map) (aValid: valid_attacker a n) (m : idMachine) (u: idUser),
+      valid_concrete_network n -> Pre a (Abuse_Elevation_Control_Mechanism m u) -> Post a (Abuse_Elevation_Control_Mechanism m u) n a' -> valid_attacker_ii a'.
+  Proof.
+    intros a a' network validAttacker m u validNetwork pre post.
+    unfold valid_attacker_ii.
+    intros m0 p0 H_secrets_a'.
+    elim_intro_clear validAttacker validAttackerI validAttacker'.
+    elim_intro_clear validAttacker' validAttackerII validAttacker''.
+    unfold Pre in pre; unfold Post in post.
+    clear validNetwork validAttacker''.
+
+    elim_intro_clear post Hsecrets post'.
+    elim_intro_clear post' Hmastered post.
+    elim_intro_clear post mac post'.
+    elim_intro_clear post' macView post.
+    elim_intro_clear post newMacView post'.
+    elim_intro_clear post' u' post.
+    elim_intro_clear post newAccountsView post'.
+    elim_intro_clear post' accHigh post.
+    elim_intro_clear post accHighView post'.
+
+    elim_intro_clear post' network_m post.
+    elim_intro_clear post env_macView post'.
+    elim_intro_clear post' Hin_accs post.
+    elim_intro_clear post HaccHigh_user post'.
+    elim_intro_clear post' HaccHigh_service post.
+    elim_intro_clear post HaccHigh_priv post'.
+    elim_intro_clear post' HaccHighView_eq post.
+    elim_intro_clear post newAccountsView_eq post'.
+    elim_intro_clear post' newMacView_eq post.
+    elim_intro_clear post known_machines_a' env_a'.
+
+    unfold valid_attacker_ii in validAttackerII.
+    elim (validAttackerII m0 p0).
+    intros MAC IH.
+    elim_intro_clear IH env_MAC path_MAC.
+    - case (idMachine_eq m0 m); intro eq_m0.
+      -- exists newMacView.
+         split.
+         --- rewrite env_a'.
+             unfold modify_machine.
+             case (idMachine_eq m0 m); intros.
+             ---- reflexivity.
+             ---- contradiction.
+         --- unfold registered_paths.
+             rewrite newMacView_eq.
+             simpl.
+             assert (macView = MAC).
+             ---- apply (enviroment_map_image (enviroment a) m macView MAC).
+                  ----- exact env_macView.
+                  ----- rewrite <- eq_m0. exact env_MAC.
+             ---- rewrite <- H in path_MAC.
+                  unfold registered_paths in path_MAC.
+                  exact path_MAC.
+      -- exists MAC.
+         rewrite (enviroment_eq (enviroment a) (enviroment a') m0 m newMacView).
+         --- split.
+             ---- exact env_MAC.
+             ---- exact path_MAC.
+         --- exact eq_m0.
+         --- exact env_a'.
+    - rewrite Hsecrets in H_secrets_a'.
+      exact H_secrets_a'.
+  Qed.
