Invariant/ValidAttacker/ValidAttackerIII/AbuseElevationControlMechanism.v
@@ -1,0 +1,160 @@
+Require Import Coq.Lists.List.
+
+Require Import Machine.Machine.
+Require Import Machine.MachineValid.
+Require Import Machine.MachineAuxFunctions.
+Require Import Attacker.Attacker.
+Require Import Technique.Technique.
+Require Import Technique.TechniquePreCondition.
+Require Import Technique.TechniquePostCondition.
+
+Require Import Invariant.AuxLemmas.AuxLemmasEnviroment.
+Require Import Invariant.AuxLemmas.AuxLemmasAccount.
+Require Import Invariant.AuxTactics.
+
+Lemma one_step_abuse_elevation_control_mechanism_preserves_valid_attacker_iii : forall (a a' : Attacker) (n: network_map) (aValid: valid_attacker a n) (m : idMachine) (u: idUser),
+      valid_concrete_network n -> Pre a (Abuse_Elevation_Control_Mechanism m u) -> Post a (Abuse_Elevation_Control_Mechanism m u) n a' -> valid_attacker_iii a'.
+  Proof.
+    intros a a' network validAttacker m u validNetwork pre post.
+    unfold valid_attacker_iii.
+    unfold valid_network.
+    elim_intro_clear validAttacker validAttackerI validAttacker'.
+    elim_intro_clear validAttacker' validAttackerII validAttacker''.
+    elim_intro_clear validAttacker'' validAttackerIII validAttackerIV.
+    unfold Pre in pre; unfold Post in post.
+    clear validNetwork validAttackerI validAttackerII validAttackerIV.
+
+    elim_intro_clear post Hsecrets post'.
+    elim_intro_clear post' Hmastered post.
+    elim_intro_clear post mac post'.
+    elim_intro_clear post' macView post.
+    elim_intro_clear post newMacView post'.
+    elim_intro_clear post' u' post.
+    elim_intro_clear post newAccountsView post'.
+    elim_intro_clear post' accHigh post.
+    elim_intro_clear post accHighView post'.
+
+    elim_intro_clear post' network_m post.
+    elim_intro_clear post env_macView post'.
+    elim_intro_clear post' Hin_accs post.
+    elim_intro_clear post HaccHigh_user post'.
+    elim_intro_clear post' HaccHigh_service post.
+    elim_intro_clear post HaccHigh_priv post'.
+    elim_intro_clear post' HaccHighView_eq post.
+    elim_intro_clear post newAccountsView_eq post'.
+    elim_intro_clear post' newMacView_eq post.
+    elim_intro_clear post known_machines_a' env_a'.
+
+    unfold valid_attacker_iii in validAttackerIII.
+    unfold valid_network in validAttackerIII.
+    elim_intro_clear validAttackerIII network_top_enva valid_machine_enva.
+    unfold network_topology in *.
+    split.
+    - intros.
+      rewrite env_a'.
+      unfold modify_machine.
+      case (idMachine_eq neighbour m); case (idMachine_eq mid m); intros eq_mid eq_neigh.
+      -- exists newMacView; auto.
+      -- exists newMacView; auto.
+      -- apply (network_top_enva m neighbour macView).
+         --- intro contra. symmetry in contra. exact (eq_neigh contra).
+         --- exact env_macView.
+         --- assert (Hmacm0_eq: m0 = newMacView).
+             ---- apply (enviroment_simpl (enviroment a) (enviroment a') mid m).
+                  ----- exact eq_mid.
+                  ----- exact env_a'.
+                  ----- exact H0.
+             ---- rewrite Hmacm0_eq in H1.
+                  rewrite newMacView_eq in H1.
+                  unfold is_neighbour in *.
+                  simpl in H1.
+                  exact H1.
+      -- apply (network_top_enva mid neighbour m0).
+         --- exact H.
+         --- rewrite <- (enviroment_eq (enviroment a) (enviroment a') mid m newMacView).
+             ---- exact H0.
+             ---- exact eq_mid.
+             ---- exact env_a'.
+         --- exact H1.
+    - intros.
+      case (idMachine_eq mid m); intros eq_m.
+      -- assert (Hmacm0_eq: m0 = newMacView).
+         apply (enviroment_simpl (enviroment a) (enviroment a') mid m).
+         --- exact eq_m.
+         --- exact env_a'.
+         --- exact H.
+         --- rewrite Hmacm0_eq.
+             elim (valid_machine_enva m macView).
+             intros.
+             elim_intro_clear H1 Husers_services_macView H1'.
+             elim_intro_clear H1' Hexploits_macView HvalidfileSystem_macView.
+             unfold valid_machine.
+             rewrite newMacView_eq.
+             split.
+             ---- unfold users_access_to_files in *.
+                  unfold registered_users in *.
+                  simpl.
+                  rewrite newAccountsView_eq.
+                  intros f Hinf.
+                  destruct (H0 f Hinf) as [Hacc_user H5].
+                  destruct H5 as [ Hacc Hin_f].
+                  destruct Hacc as [acc Hacc'].
+                  destruct Hacc' as [ Heq_acc Hin_acc ].
+                  case (idUser_eq Hacc_user u'); intros Heq_u0.
+                  ----- exists Hacc_user.
+                        split.
+                        ------ exists accHighView.
+                              split.
+                              ------- rewrite HaccHighView_eq. simpl. symmetry. exact Heq_u0.
+                              ------- apply member_addAccount. auto.
+                        ------ exact Hin_f.
+                  ----- exists Hacc_user.
+                        split.
+                        ------ exists acc.
+                              split.
+                              ------- exact Heq_acc.
+                              ------- apply addAccount_preserves_membership_when_neq.
+                                    -------- rewrite Heq_acc. rewrite HaccHighView_eq. simpl. exact Heq_u0.
+                                    -------- exact Hin_acc.
+                        ------ exact Hin_f.
+             ---- split.
+                  ----- unfold users_access_to_services in *.
+                        unfold registered_service in *.
+                        rewrite newAccountsView_eq.
+                        simpl.
+                        intros acc0 HIP.
+                        apply member_addAccount_simpl in HIP.
+                        destruct HIP as [HIP_eq | HIP_in].
+                        ------ rewrite <- HIP_eq.
+                               rewrite HaccHighView_eq.
+                               simpl.
+                               right.
+                               exists OS.
+                               split. reflexivity.
+                               destruct pre as [_ [accPre [macPre [kPre [HenvPre [HinPre_acc [_ [HservPre _]]]]]]]].
+                               rewrite (enviroment_map_image _ _ _ _ HenvPre env_macView) in HinPre_acc.
+                               destruct (Husers_services_macView accPre HinPre_acc) as [Hno_serv | [s [Hs_eq Hreg]]].
+                               ------- rewrite HservPre in Hno_serv. discriminate.
+                               ------- rewrite HservPre in Hs_eq.
+                                       injection Hs_eq as Hs_eq'.
+                                       rewrite Hs_eq'.
+                                       exact Hreg.
+                        ------ apply Husers_services_macView. exact HIP_in.
+                  ----- unfold valid_fileSystem in *.
+                        unfold exploits_services in *.
+                        unfold registered_service in *.
+                        unfold subfiles_in_machine in *.
+                        unfold registered_paths in *.
+                        simpl.
+                        split.
+                        ------ exact Hexploits_macView.
+                        ------ exact HvalidfileSystem_macView.
+             ---- exact env_macView.
+      -- assert (Henv_eq: enviroment a' mid = enviroment a mid).
+         apply (enviroment_eq (enviroment a) (enviroment a') mid m newMacView).
+         --- exact eq_m.
+         --- exact env_a'.
+         --- rewrite Henv_eq in H.
+             apply (valid_machine_enva mid m0).
+             exact H.
+  Qed.
