Invariant/ValidAttacker/ValidAttackerIII/NetworkServiceScanning.v
@@ -1,0 +1,152 @@
+Require Import Coq.Lists.List.
+
+Require Import Machine.Machine.
+Require Import Machine.MachineValid.
+Require Import Machine.MachineAuxFunctions.
+Require Import Attacker.Attacker.
+Require Import Technique.Technique.
+Require Import Technique.TechniquePreCondition.
+Require Import Technique.TechniquePostCondition.
+
+Require Import Invariant.AuxLemmas.AuxLemmasEnviroment.
+Require Import Invariant.AuxLemmas.AuxLemmasService.
+Require Import Invariant.AuxTactics.
+
+Lemma one_step_network_service_scanning_preserves_valid_attacker_iii : forall (a a' : Attacker) (n: network_map) (aValid: valid_attacker a n) (m m': idMachine) (u : idUser) (l: list nat),
+      valid_concrete_network n -> Pre a (Network_Service_Scanning m u m' l) -> Post a (Network_Service_Scanning m u m' l) n a' -> valid_attacker_iii a'.
+  Proof.
+    intros a a' network validAttacker m m' u l validNetwork pre post.
+    unfold valid_attacker_iii; unfold valid_network.
+    unfold Pre in pre; unfold Post in post.
+    elim_intro_clear validAttacker validAttackerI validAttacker'.
+    elim_intro_clear validAttacker' validAttackerII validAttacker''.
+    elim_intro_clear validAttacker'' validAttackerIII validAttacker'''.
+    clear validAttackerI validAttackerII validAttacker'''.
+
+    elim_intro_clear post Hknown_machines post'.
+    elim_intro_clear post' Hsecrets post.
+    elim_intro_clear post Hmastered post'.
+    elim_intro_clear post' mac post.
+    elim_intro_clear post macView' post'.
+    elim_intro_clear post' newMacView' post.
+    elim_intro_clear post portsServices post'.
+    elim_intro_clear post' servicesNewView post.
+    elim_intro_clear post env_m post'.
+    elim_intro_clear post' network_m post.
+    elim_intro_clear post portsServices_eq post'.
+    elim_intro_clear post' servicesNewView_eq post.
+    elim_intro_clear post newMacView_eq env_a'.
+
+
+        unfold valid_attacker_iii in validAttackerIII.
+    unfold valid_network in validAttackerIII.
+    elim_intro_clear validAttackerIII network_top_enva valid_machine_enva.
+    unfold network_topology in *.
+
+    split.
+    - intros.
+      rewrite env_a'.
+      unfold modify_machine.
+      case (idMachine_eq neighbour m'); case (idMachine_eq mid m'); intros eq_mid eq_neigh.
+      -- exists newMacView'; auto.
+      -- exists newMacView'; auto.
+      -- apply (network_top_enva m' neighbour macView').
+         --- intro contra. symmetry in contra. exact (eq_neigh contra).
+         --- exact env_m.
+         --- assert (Hm0: m0 = newMacView').
+             ---- apply (enviroment_simpl (enviroment a) (enviroment a') mid m').
+                  ----- exact eq_mid.
+                  ----- exact env_a'.
+                  ----- exact H0.
+             ---- rewrite Hm0 in H1.
+                  rewrite newMacView_eq in H1.
+                  unfold is_neighbour in *.
+                  simpl in H1.
+                  exact H1.
+      -- apply (network_top_enva mid neighbour m0).
+         --- exact H.
+         --- rewrite <- (enviroment_eq (enviroment a) (enviroment a') mid m' newMacView').
+             ---- exact H0.
+             ---- exact eq_mid.
+             ---- exact env_a'.
+         --- exact H1.
+    - intros m0 mac' enva'_m'.
+      case (idMachine_eq m0 m'); intros eq_m0.
+      -- assert (mac' = newMacView').
+         apply (enviroment_simpl (enviroment a) (enviroment a') m0 m' mac' newMacView').
+         --- exact eq_m0.
+         --- exact env_a'.
+         --- exact enva'_m'.
+         --- rewrite H.
+             elim (valid_machine_enva m' macView').
+             ---- intros users_macView HI.
+                  elim_intro_clear HI users_services_macView HI'.
+                  elim_intro_clear HI' exploits_macView fileSystem_macView.
+                  unfold valid_machine.
+                  rewrite newMacView_eq.
+                  split.
+                  ------ unfold users_access_to_files in *.
+                         unfold registered_users in *.
+                         simpl.
+                         exact users_macView.
+                  ------ split.
+                         ------- unfold users_access_to_services in *.
+                                 unfold registered_service in *.
+                                 simpl.
+                                 rewrite servicesNewView_eq.
+                                 intros acc Hinacc.
+                                 elim (users_services_macView acc).
+                                 -------- intro Hnone. left. exact Hnone.
+                                 -------- intros [s [Heq_s [service [Heq_service H_in_service]]]].
+                                          right. exists s. split.
+                                          --------- exact Heq_s.
+                                          --------- exists service. split.
+                                                    ---------- exact Heq_service.
+                                                    ---------- rewrite portsServices_eq.
+                                                               apply oplusServices_preserves_membership.
+                                                               exact H_in_service.
+                                 -------- exact Hinacc.
+                         ------- split.
+                                 -------- unfold exploits_services in *.
+                                          unfold registered_service in *.
+                                          simpl.
+                                          intros s0 e0 Hin_exploits.
+                                          rewrite servicesNewView_eq.
+                                          elim (exploits_macView s0 e0).
+                                          --------- intros serv HI.
+                                                    elim_intro_clear HI serv_value_eq H_in_service.
+                                                    exists serv.
+                                                    split.
+                                                    ---------- exact serv_value_eq.
+                                                    ---------- rewrite portsServices_eq.
+                                                               apply oplusServices_preserves_membership.
+                                                               exact H_in_service.
+                                          --------- exact Hin_exploits.
+                                 -------- unfold valid_fileSystem in *.
+                                          simpl.
+                                          elim_intro_clear fileSystem_macView subfiles_macView fileSystem'_macView.
+                                          split.
+                                          --------- unfold subfiles_in_machine in *.
+                                                    unfold registered_paths in *.
+                                                    simpl.
+                                                    exact subfiles_macView.
+                                          --------- exact fileSystem'_macView.
+             ---- exact env_m.
+      -- elim (valid_machine_enva m0 mac').
+         --- intros users_mac' HI.
+            elim_intro_clear HI subfiles_mac' HI'.
+            elim_intro_clear HI' users_services_mac' unique_mac'.
+            unfold valid_machine.
+            split.
+            ---- exact users_mac'.
+            ---- split.
+                 ------ exact subfiles_mac'.
+                 ------ unfold valid_fileSystem.
+                        split.
+                        -------- exact users_services_mac'.
+                        -------- exact unique_mac'.
+         --- rewrite <- (enviroment_eq (enviroment a) (enviroment a') m0 m' newMacView').
+             ---- exact enva'_m'.
+             ---- exact eq_m0.
+             ---- exact env_a'.
+  Qed.
