Invariant/ValidAttacker/ValidAttackerIV/AbuseElevationControlMechanism.v
@@ -1,0 +1,137 @@
+Require Import Coq.Lists.List.
+
+Require Import Machine.Machine.
+Require Import Machine.MachineValid.
+Require Import Machine.MachineAuxFunctions.
+Require Import Machine.MachineView.
+
+Require Import Attacker.Attacker.
+
+Require Import Technique.Technique.
+Require Import Technique.TechniquePreCondition.
+Require Import Technique.TechniquePostCondition.
+
+Require Import Invariant.AuxLemmas.AuxLemmasEnviroment.
+Require Import Invariant.AuxLemmas.AuxLemmasAccount.
+Require Import Invariant.AuxTactics.
+
+Lemma one_step_abuse_elevation_control_mechanism_preserves_valid_attacker_iv : forall (a a' : Attacker) (n: network_map) (aValid: valid_attacker a n) (m : idMachine) (u: idUser),
+      valid_concrete_network n -> Pre a (Abuse_Elevation_Control_Mechanism m u) -> Post a (Abuse_Elevation_Control_Mechanism m u) n a' -> valid_attacker_iv a' n.
+  Proof.
+    intros a a' network validAttacker m u validNetwork pre post.
+    unfold valid_attacker_iv.
+    unfold is_networkView.
+    elim_intro_clear validAttacker validAttackerI validAttacker'.
+    elim_intro_clear validAttacker' validAttackerII validAttacker''.
+    elim_intro_clear validAttacker'' validAttackerIII validAttackerIV.
+    unfold Pre in pre; unfold Post in post.
+    clear validAttackerI validAttackerII validAttackerIII.
+
+    elim_intro_clear post Hsecrets post'.
+    elim_intro_clear post' Hmastered post.
+    elim_intro_clear post mac post'.
+    elim_intro_clear post' macView post.
+    elim_intro_clear post newMacView post'.
+    elim_intro_clear post' u' post.
+    elim_intro_clear post newAccountsView post'.
+    elim_intro_clear post' accHigh post.
+    elim_intro_clear post accHighView post'.
+
+    elim_intro_clear post' network_m post.
+    elim_intro_clear post env_macView post'.
+    elim_intro_clear post' Hin_accs post.
+    elim_intro_clear post HaccHigh_user post'.
+    elim_intro_clear post' HaccHigh_service post.
+    elim_intro_clear post HaccHigh_priv post'.
+    elim_intro_clear post' HaccHighView_eq post.
+    elim_intro_clear post newAccountsView_eq post'.
+    elim_intro_clear post' newMacView_eq post.
+    elim_intro_clear post known_machines_a' env_a'.
+
+    unfold valid_attacker_iv in validAttackerIV.
+    unfold is_networkView in validAttackerIV.
+    intros m0 mac1 mac2 env_a'_m0 network_m0.
+    unfold is_machineView.
+    case (idMachine_eq m0 m); intros eq_m0.
+    elim (validAttackerIV m0 macView mac).
+    intros Hserv. intro Hserv'.
+    destruct Hserv' as [Haccs Hserv''].
+    destruct Hserv'' as [Hfiles Hserv'''].
+    destruct Hserv''' as [Hneighs Hexploits].
+    assert (Heq_mac1: mac1 = newMacView).
+    {
+      apply (enviroment_simpl (enviroment a) (enviroment a') m0 m mac1 newMacView).
+      - exact eq_m0.
+      - exact env_a'.
+      - exact env_a'_m0.
+    }
+    assert (Heq_mac2: mac2 = mac).
+    {
+      apply (enviroment_map_image network m mac2 mac).
+      - rewrite eq_m0 in network_m0. exact network_m0.
+      - exact network_m.
+    }
+    rewrite Heq_mac1.
+    rewrite Heq_mac2.   
+    split; [|split; [|split]]; try split.
+    - unfold subset_services in *.
+      rewrite newMacView_eq.
+      simpl.
+      exact Hserv.
+    - unfold subset_accounts in *.
+      rewrite newMacView_eq.
+      simpl.
+      rewrite newAccountsView_eq.
+      intros Hacc Hin_addAccount.
+      assert (Hin_Hacc: accHighView = Hacc \/ In Hacc (machine_accounts macView)).
+      {
+        apply (member_addAccount_simpl Hacc accHighView (machine_accounts macView)).
+        exact Hin_addAccount.
+      }
+      destruct Hin_Hacc as [Heq_Hacc | Hin_macView].
+      -- right.
+         rewrite <- Heq_Hacc.
+         exists accHigh.
+         split.
+         --- exact Hin_accs.
+         --- unfold account_view.
+             rewrite HaccHighView_eq.
+             simpl.
+             split; [ |split]; try split.
+             ---- symmetry. exact HaccHigh_user.
+             ---- right. symmetry. exact HaccHigh_service.
+             ---- left. reflexivity.
+             ---- right. symmetry. exact HaccHigh_priv.
+      -- apply (Haccs Hacc).
+         exact Hin_macView.
+    - unfold subset_files in *.
+      rewrite newMacView_eq.
+      simpl.
+      exact Hfiles.
+    - unfold subset_neighbours in *.
+      rewrite newMacView_eq.
+      simpl.
+      exact Hneighs.
+    - unfold subset_exploits in *.
+      rewrite newMacView_eq.
+      simpl.
+      exact Hexploits.
+    - rewrite <- eq_m0 in env_macView. exact env_macView.
+    - rewrite <- eq_m0 in network_m. exact network_m.
+    - elim (validAttackerIV m0 mac1 mac2).
+      intros Hserv. intro Hserv'.
+      destruct Hserv' as [Haccs Hserv''].
+      destruct Hserv'' as [Hfiles Hserv'''].
+      destruct Hserv''' as [Hneighs Hexploits].
+      split; [|split; [|split]]; try split.
+      -- exact Hserv.
+      -- exact Haccs.
+      -- exact Hfiles.
+      -- exact Hneighs.
+      -- exact Hexploits.
+      -- rewrite <- (enviroment_eq (enviroment a) (enviroment a') m0 m newMacView).
+         --- exact env_a'_m0.
+         --- exact eq_m0.
+         --- exact env_a'.
+      -- exact network_m0.
+  Qed.
