Invariant/ValidAttacker/ValidAttackerIV/NetworkServiceScanning.v
@@ -1,0 +1,113 @@
+Require Import Coq.Lists.List.
+
+Require Import Machine.Machine.
+Require Import Machine.MachineValid.
+Require Import Machine.MachineAuxFunctions.
+Require Import Machine.MachineView.
+Require Import Attacker.Attacker.
+Require Import Technique.Technique.
+Require Import Technique.TechniquePreCondition.
+Require Import Technique.TechniquePostCondition.
+
+Require Import Invariant.AuxLemmas.AuxLemmasEnviroment.
+Require Import Invariant.AuxLemmas.AuxLemmasService.
+Require Import Invariant.AuxTactics.
+
+Lemma one_step_network_service_scanning_preserves_valid_attacker_iv : forall (a a' : Attacker) (n: network_map) (aValid: valid_attacker a n) (m m': idMachine) (u : idUser) (l: list nat),
+      valid_concrete_network n -> Pre a (Network_Service_Scanning m u m' l) -> Post a (Network_Service_Scanning m u m' l) n a' -> valid_attacker_iv a' n.
+  Proof.
+    intros a a' network validAttacker m m' u l validNetwork pre post.
+    unfold valid_attacker_iv.
+    unfold is_networkView.
+    elim_intro_clear validAttacker validAttackerI validAttacker'.
+    elim_intro_clear validAttacker' validAttackerII validAttacker''.
+    elim_intro_clear validAttacker'' validAttackerIII validAttackerIV.
+    unfold Pre in pre; unfold Post in post.
+    clear validAttackerI validAttackerII validAttackerIII.
+
+    elim_intro_clear post Hknown_machines post'.
+    elim_intro_clear post' Hsecrets post.
+    elim_intro_clear post Hmastered post'.
+    elim_intro_clear post' mac post.
+    elim_intro_clear post macView' post'.
+    elim_intro_clear post' newMacView' post.
+    elim_intro_clear post portsServices post'.
+    elim_intro_clear post' servicesNewView post.
+    elim_intro_clear post env_m post'.
+    elim_intro_clear post' network_m post.
+    elim_intro_clear post portsServices_eq post'.
+    elim_intro_clear post' servicesNewView_eq post.
+    elim_intro_clear post newMacView_eq env_a'.
+
+    unfold valid_attacker_iv in validAttackerIV.
+    unfold is_networkView in validAttackerIV.
+    intros m0 mac1 mac2 env_a'_m0 network_m0.
+    unfold is_machineView.
+
+    case (idMachine_eq m0 m'); intros eq_m0.
+    elim (validAttackerIV m0 macView' mac).
+    intros Hserv. intro Hserv'.
+    destruct Hserv' as [Haccs Hserv''].
+    destruct Hserv'' as [Hfiles Hserv'''].
+    destruct Hserv''' as [Hneighs Hexploits].
+    assert (Heq_mac1: mac1 = newMacView').
+    {
+      apply (enviroment_simpl (enviroment a) (enviroment a') m0 m' mac1 newMacView').
+      - exact eq_m0.
+      - exact env_a'.
+      - exact env_a'_m0.
+    }
+    assert (Heq_mac2: mac2 = mac).
+    {
+      apply (enviroment_map_image network m' mac2 mac).
+      - rewrite eq_m0 in network_m0. exact network_m0.
+      - exact network_m.
+    }
+    rewrite Heq_mac1.
+    rewrite Heq_mac2.
+    split; [|split; [|split]]; try split.
+    - unfold subset_services in *.
+      rewrite newMacView_eq.
+      simpl.
+      rewrite servicesNewView_eq.
+      rewrite portsServices_eq.
+      intros s' Hin_oplus.
+      apply oplusServices_membership in Hin_oplus.
+      destruct Hin_oplus as [ Hin_macView | Hin_mac ].
+      -- apply Hserv. exact Hin_macView.
+      -- apply (scanServices_subset s' (machine_services mac) l). exact Hin_mac.
+    - unfold subset_accounts in *.
+      rewrite newMacView_eq.
+      simpl.
+      exact Haccs.
+    - unfold subset_files in *.
+      rewrite newMacView_eq.
+      simpl.
+      exact Hfiles.
+    - unfold subset_neighbours in *.
+      rewrite newMacView_eq.
+      simpl.
+      exact Hneighs.
+    - unfold subset_exploits in *.
+      rewrite newMacView_eq.
+      simpl.
+      exact Hexploits.
+    - rewrite <- eq_m0 in env_m. exact env_m.
+    - rewrite <- eq_m0 in network_m. exact network_m.
+    - elim (validAttackerIV m0 mac1 mac2).
+      intros Hserv. intro Hserv'.
+      destruct Hserv' as [Haccs Hserv''].
+      destruct Hserv'' as [Hfiles Hserv'''].
+      destruct Hserv''' as [Hneighs Hexploits].
+      split; [|split; [|split]]; try split.
+      -- exact Hserv.
+      -- exact Haccs.
+      -- exact Hfiles.
+      -- exact Hneighs.
+      -- exact Hexploits.
+      -- rewrite <- (enviroment_eq (enviroment a) (enviroment a') m0 m' newMacView').
+         --- exact env_a'_m0.
+         --- exact eq_m0.
+         --- exact env_a'.
+      -- exact network_m0.
+  Qed.
